\documentclass{standalone}

\usepackage{amsmath}
\usepackage{hyphenat}
\usepackage{xspace}

\begin{document}
\subsection {Aufgabe 9.5}
\begin{itemize}
    \item[a)]
    $\int_{\pi/6}^{\pi/2}\frac{x}{\sin^2(x)}\,dx$=
    $\begin{pmatrix}
    f = x & f' = 1 \\
    g' = \frac{1}{\sin^2(x)} & g = -\cot(x)
    \end{pmatrix}$\\
    =$x(- cot(x))\mid^{\pi/2}_{\pi/6}$-$\int_{\pi/6}^{\pi/2}-\cot(x) \,dx$\\
    =$x(- cot(x))\mid^{\pi/2}_{\pi/6}$+$\int_{\pi/6}^{\pi/2}\cot(x) \,dx$=
    $x(- cot(x))\mid^{\pi/2}_{\pi/6}$$\ln(\sin(x))\mid^{\pi/2}_{\pi/6}$\\
    =$\frac{\pi}{2}*0+\frac{\pi}{6}+1-\ln(\frac{1}{2})$=
    $\frac{\pi}{6}\cot(\frac{\pi}{6})+1-\ln(1)+\ln(2)$

    \item[b)]
    $\int_{0}^{1}r^2\sqrt{1-r} \,dx$=
    $\begin{pmatrix}
    t = 1-r & \\
        \frac{dt}{dx} = -1 & dx = -dt
        \end{pmatrix}$=
    $\int_{0}^{1}\sqrt{t}(1-t)^2 \,dx$=
    $\int_{0}^{1}t^{\frac{1}{2}}(t^2-2t+1) \,dx$=
    $\int_{0}^{1}t^{\frac{5}{2}}-2t^{\frac{3}{2}}+t^{\frac{1}{2}} \,dx$=
    $\int_{0}^{1}t^{\frac{5}{2}}\,dx-\int_{0}^{1}2t^{\frac{3}{2}}\,dx+\int_{0}^{1}t^{\frac{1}{2}} \,dx$=+
    $-\frac{2(t)^{\frac{7}{2}}}{7}+\frac{4(t)^{\frac{5}{2}}}{5}-\frac{2(t)^{\frac{3}{2}}}{3}$
    $\frac{2(42(r-1)^{\frac{7}{2}}+15(x-1)^{\frac{5}{2}}+35)(1-x)^{\frac{3}{2}}}{105}$+C=
    F(1)-F(0)=$-\frac{2(35)(0)}{105}-(-\frac{2(-42+15+35)(1)^{\frac{3}{2}}}{105})$=
    $+\frac{2(8)}{105}$= $\frac{16}{105}$
    \item[c)]
    $\int_{0}^{1}\frac{e^x}{(1+e^x)^2} \,dx$=
    $\begin{pmatrix}
        t = 1+e^x &  \\
        \frac{dt}{dx} = e^x & dx = \frac{dt}{e^x}
    \end{pmatrix}$\\
    =$\int_{0}^{1}\frac{e^x}{(1+e^x)^2} \,\frac{dt}{e^x}$=
    $-\frac{1}{t}$+C=
    $-\frac{1}{1+e^x}$+C\\
    =F(1)-F(0)=$-\frac{1}{1+e^1}-(-\frac{1}{1+e^0})$=$\frac{1}{2}-\frac{1}{1+e^1}$=
    $\frac{1+e^1-2}{2(1+e^1)}$=$\frac{e^1-1}{2+2e^1}$

    \item[d)]
    $\int\frac{\cos{\ln(x)}}{x} \,dx$=
    $\begin{pmatrix}
        t = \ln(x) &  \\
        \frac{dt}{dx} = \frac{1}{x} & dx = dtx
    \end{pmatrix}$= 
    $\int_{0}^{1}\frac{\cos{t}}{x} \,(x*dt)$=
    $\sin(t)$=$\sin\ln(x)$

    \item[e)]
    $\int \cos(e^{\sin(x)})*e^{\sin(x)}*\cos(x)\,dx$=
    $\begin{pmatrix}
        t = e^{\sin(x)} &  \\
        \frac{dt}{dx} = \cos(x)e^{sin(x)} & dx = \frac{dt*e^{-sin(x)}}{\cos(x)}
    \end{pmatrix}$\\
    =$\int \cos(t)*e^{\sin(x)}*\cos(x)*\frac{e^{-sin(x)}}{\cos(x)}\,dt$= 
    $\int \cos(t)\,dt$\\
    $=\sin(t)$=$\sin(e^{\sin(x)})+C$

    \item[f)]
    $\int \frac{e^x}{e^x+e^{-x}}\,dx$=
    $\begin{pmatrix}
        t = e^x &  \\
        \frac{dt}{dx} = e^x & dx = \frac{dt}{e^x}  
    \end{pmatrix}$=
    $\int \frac{t}{t+\frac{1}{e^-x}}\,dx$\\
    =$\int \frac{t}{t+\frac{1}{t}}\,dx$=
    $\int \frac{t*t}{t}\,dx$=$\int t \,dx$=$\frac{t^2}{2}$ Wir ersetzen T zurück$\rightarrow$
    $\frac{ln^3(x)}{3}+C$

    \item[g)]   
    $\int \frac{ln^2(x)}{x}\,dx=
    \begin{pmatrix}
        t = \ln(x) &  \\
        \frac{dt}{dx} = \frac{1}{x} & dx = xdt  
    \end{pmatrix}=$
    $\int \frac{t^2}{x}\,(x*dt)=\int t\,dx=\frac{t^3}{3}$ Wir ersetzen T zurück$\rightarrow$
    $\frac{ln^3(x)}{3}+C$


\end{itemize}
\end{document}
