\documentclass{standalone}
\begin{document}
\subsection{Aufgabe 12.2}

	
a ) $ (1 + 4i ) (2- 3i ) = 14 + 5 i $

b ) $\frac{4}{2i} = \frac{8}{5} - \frac{4}{5} i $

c ) $\sum\limits_{n=0}^{2020} i^n = 1 $, da $i^0 = 1 $


\subsection{Aufgabe 12.3}

1 ) $ (1 + 2i) + 3 (1 + 2i)^2 + 2 (1 + 2i) = 0 - 10i $ 
	
	2 ) $ \frac{(1+2i)+(-2+i)}{4(\frac{(1-i)}{2}) - (-2+i)} = - \frac{13}{25} + \frac{9}{25}i $ 
	
	3 ) $ \frac{(-2+i)^2}{2(1+2i)+2(\frac{1-i}{2})+i} = \frac{6}{25}+0i$
	
	
	Gleichung: 
	
	
	$z-1+2iz-i=0$ 
	
	$ a+bi-1+2ai+2b-i=0$
	
	$ a+2b-1+(b+2a-1)i=0 $
	
	Daraus erhält man: $ a+2b=1 $ und $2a+b=1$, also $ 3a+3b=2 $ somit gilt 
	
	$ a+b=\frac{2}{3}$ , wobei $a=\frac{1}{3}$, $b=\frac{1}{3}$	
	
	Damit ist $ Z=\frac{1}{3}+\frac{1}{3}i$ die Lösung. 

\end{document}
