\documentclass{standalone}
\begin{document}
\subsection{Aufgabe 8.3}


a) $ p_1= x^3 - 2x - 1  = (x+1)(x^2 -x -1)  $


b) $ p_2 = x^4 - 3x^3 - 3x^2 +11x - 6 = (x-1)^2 (x-3) (x + 2) $


c) $p_3= x^4 - 6x^2 + 7 = (x-\sqrt{3+\sqrt2}) (x-\sqrt{3-\sqrt2}) (x+\sqrt{3+\sqrt2})\\\indent\indent\indent(x+\sqrt{3-\sqrt2})$

d) $ p_4 = 9x^4 + 30x^3 + 16x^2 -30x - 25= 3 (3x+5)(x+\frac{5}{3})(x+1)(x-1)$

e) $ p_5= x^3-7x^2+4x+12= (x+1)(x-2)(x-6)$

f) $p_6= x^4+x^3+2x^2+x+1= (x^2+1)(x^2+x+1)$

g) $p_7= x^4+4x^3+2x^2-4x-3=(x+1)^2(x-1)(x+3)$

h) $p_8= x^3+1= (x^2-x+1)(x+1)$

i) $p_9= 2x^3+3x+5= (x+1)(2x^2-2x+5)$

\end{document}