\documentclass{standalone}
\begin{document}
\subsection{Aufgabe 11.4}
<<<<<<< HEAD
\begin{enumerate}[a)]
    \item \begin{align}
        y' &= -\frac{x}{y} \\
        y'y &= -x \\
        y^2 &= -x^2 + c \\
        y &= \sqrt{c-x^2}
        y(1) &= 1 \text{ einsetzen} \\
        1 &= \sqrt{c-1} \\
        c &= 2 \\
        \rightarrow y = \sqrt{2-x^2}
    \end{align}
    \item \begin{align}
        y' &= e^y\sin x \\
        \frac{y'}{e^y} &= sin x \\
        \int \frac{1}{u^2}du &= \int sin x dx \text{, mit } u = e^y, du = y'e^y = y'u \\
        -\frac{1}{e^y} &= -\cos x + c \\
        y &= \ln \frac{1}{\cos x - c}
        y(0) = 0 \text{ einsetzen} \\
        0 &= \ln \frac{1}{1-c} \\
        1 &= \frac{1}{1-c} \\
        c &= 0 \\
        \rightarrow y &= \ln \frac{1}{\cos x}
    \end{align}
    \item \begin{align}
        x^2 y &= (1+x)y' \\
        \frac{y'}{y} &= \frac{x^2}{1+x} \text{, Polynomdivision} \\
        \int \frac{y'}{y}dy &= \int x - 1 + \frac{1}{1+x}dx \\
        y &= e^{\frac{1}{2}x^2 - x + \ln (1+x)} + c \\
        y(0) &= 1 \text{ einsetzen} \\
        1 &= 1 + c\\
        c &= 0 \\
        \rightarrow y &= e^{\frac{1}{2}x^2 - x + \ln (1+x)}
    \end{align}
\end{enumerate}

\end{document}
