\documentclass{standalone}
\begin{document}
\subsection{Aufgabe 13.2}

a)\\
exp$\left(i*\frac{\pi}{6}\right)=\frac{\sqrt{3}}{2}+\frac{i}{2}$\\ 
exp$\left(-\frac{5\pi}{3i}\right)=$exp$\left(\frac{\pi*i}{3}\right)=\frac{1}{2}+\frac{\sqrt{3}}{2}*i$\\

\noindent b)\\
exp$\left(i*\frac{\pi}{4}\right)=\frac{\sqrt{2}}{2}+\frac{\sqrt{2}}{2}*i$\\
exp$\left(-i*\frac{\pi}{4}\right)=\frac{\sqrt{2}}{2}-\frac{\sqrt{2}}{2}*i$\\
exp$\left(-i*\frac{\pi}{4}\right)*$exp$\left(i*\frac{\pi}{4}\right)=1$\\


\subsection{Aufgabe 13.3}

a)\\
$z=\frac{-2}{1+\sqrt{3}*i} \implies z=-\frac{1}{2}+\frac{\sqrt{3}}{2}*i\\
\abs{z}=1\\
-\frac{1}{2}=cos(\varphi) \leftrightarrow \varphi = \pm \frac{2}{3}\pi\\
\frac{\sqrt{3}}{2}=sin(\varphi) \leftrightarrow \varphi = \frac{2}{3}\pi\\
z=cos\left(\frac{2}{3}\pi \right) + i * sin\left(\frac{2}{3}\pi \right)$\\


\noindent b)\\ 
$z= \frac{i}{-2-2i} \implies z=-\frac{1}{4}-\frac{1}{4}*i\\
\abs{z}=\frac{\sqrt{2}}{4}\\
-\frac{1}{\sqrt{2}}=cos(\varphi) \leftrightarrow \varphi = \pm \frac{3}{4}\pi\\
-\frac{1}{\sqrt{2}}=sin(\varphi) \leftrightarrow \varphi = -\frac{3}{4}\pi\\
z=\frac{\sqrt{2}}{4}*\left(cos\left(-\frac{3}{4}\pi \right)+ i * sin\left(-\frac{3}{4} \pi \right)\right)$
 

\end{document}
