\documentclass{standalone}
\begin{document}
\subsection{Aufgabe 9.7}

\begin{enumerate}[a)]
    \item \begin{align}
        \int f(x) &= \int \tan x dx \\
        F(x) &= \int \tan x  dx \\
        &= \int \frac{\sin x}{\cos x} dx \\
        &= \int -\frac{1}{u} du \text{, mit } u = cos x, du = -sin x dx \\
        &= -\int \frac{1}{u} du \\
        &= - (\ln u + c) \\
        &= \ln \frac{1}{u} - c \text{, u einsetzen} \\
        &= \ln \frac{1}{\sin x} - c
    \end{align}
    \item \begin{align}
        \int f(x) &= \int xe^{-x^2} dx \\
        F(x) &= \int xe^{-x^2} dx \\
        &= \int -\frac{1}{2}e^{u} du \text{, mit } u = -x^2, du = -2x \\
        &= -\frac{1}{2} \int e^{u} du \\
        &= -\frac{1}{2} (e^{u} + c) \text{, u einsetzen} \\
        &= -\frac{1}{2} (e^{-x^2} + c)
    \end{align}
    \item \begin{align}
        \int f(x) &= \int e^{\sqrt{2x+1}} dx \\
        F(x) = &= \int e^{\sqrt{2x+1}} dx\\
        &= \int 2e^{u}u du \text{, mit } u = \sqrt{2x+1}, dx = {2\sqrt{2x+1} du
        &= 2 \cdot ( \left[ e^{u}u \right] - \int e^{u} du + c_1) \\
        &= 2 \cdot ( \left[ e^{u}u \right] - e^{u} + c_2) \text{, u einsetzen} \\
        &= 2 \cdot (e^{u}u - e^{u} + c_2)
    \end{align}
    % \item \begin{align}
    %     g'(x) &= (\tan \frac{x}{2})' \\
    %     &= (\frac{\sin \frac{x}{2}}{\cos \frac{x}{2}})' \\
    %     &= (-\sin^2)
    % \end{align}
\end{enumerate}


\end{document}