\documentclass{standalone}
\begin{document}
\subsection{Aufgabe 11.2}
\begin{enumerate}[a)]
\item
    \begin{align*}
        \frac{dy}{dx} &= \frac{2x}{x^2+1}y \\
        \int \frac{1}{y} \,dy &= \int \frac{2x}{x^2+1} \,dx \\
        \ln|y| &= \int \frac{1}{u} \,du,\ u = x^2+1,\ u' = 2x \\
        \ln|y| &= \ln|u| + c \\
        \ln|y| &= \ln|x^2+1| + c \\
        \ln|y| &= \ln|e^c(x^2+1)| \\
        y &= e^c(x^2+1) \\
        y &= c(x^2+1) \\
    \end{align*}

\item
    \begin{align*}
        \frac{dy}{dx} (y + 1)^2 + x^3 &= 0 \\
        \int (y + 1)^2 \,dy &= \int -x^3 \,dx \\
        \frac{(y + 1)^3}{3} &= \frac{-x^4}{4} + c \\
        (y + 1)^3 &= \frac{-3x^4}{4} + c \\
        y &= \sqrt[3]{\frac{-3x^4}{4} + c} - 1 \\
    \end{align*}

\item
    \begin{align*}
        y(1-x) \frac{dy}{dx} &= 1-y^2 \\
        \int \frac{y}{1-y^2} \,dy &= \int \frac{1}{1-x} \,dx \\
        \frac{-1}{2} \int \frac{-2y}{1-y^2} \,dy &= \int \frac{1}{1-x} \,dx \\
        \frac{-1}{2} \int \frac{1}{u} \,du &= -\ln|1-x| + c,\ u = 1-y^2,\ u' = -2y \\
        \frac{1}{2} \ln|u| &= \ln|1-x| + c \\
        \ln|1-y^2| &= \ln|(e^c(1-x))^2| \\
        1-y^2 &= c(1-x)^2 \\
        y &= \sqrt{c(1-x)^2 + 1} \\
    \end{align*}

\end{enumerate}
\end{document}
